examples/mw/MWApp01proof.v
@@ -16,7 +16,7 @@ From ExtLib Require Import
      Structures.Maps
      Data.Map.FMapAList.
 
-Require Import HTactics ProofMode.
+Require Import HTactics ProofMode STB.
 
 Set Implicit Arguments.
 
@@ -32,13 +32,10 @@ Section SIMMODSEM.
   Let W: Type := Any.t * Any.t.
 
   Let wf: _ -> W -> Prop :=
-    (* @mk_wf *)
-    (*   _ *)
-    (*   unit *)
-    (*   (fun _ _ st_tgt => ((OwnM(AppInitX) ∧ ⌜st_tgt = false↑⌝) ∨ (OwnM(AppRunX) ∧ ⌜st_tgt = true↑⌝))%I) *)
-
-    fun (_: unit) '(mpr_src, mpr_tgt) => (mpr_src = (InitX)↑ ∧ mpr_tgt = false↑) ∨
-                                         (mpr_src = (RunX)↑ ∧ mpr_tgt = true↑)
+    @mk_wf
+      _
+      unit
+      (fun _ _ st_tgt => ((OwnM(Run) ∧ ⌜st_tgt = false↑⌝) ∨ (OwnM(Init) ∧ ⌜st_tgt = true↑⌝))%I)
   .
 
   Theorem correct: refines2 [MWApp0.App] [MWApp1.App].
@@ -46,67 +43,39 @@ Section SIMMODSEM.
     eapply adequacy_local2. econs; ss.
     i. econstructor 1 with (wf:=wf) (le:=top2); et; swap 2 3.
     { ss. }
-    { esplits. econs; ss. }
+    { esplits. econs; ss. eapply to_semantic. iIntros "H". iSplits; ss; et. }
 
     econs; ss.
-    { init. steps. unfold initF, MWApp0.initF, ASSUME, GUARANTEE. steps.
-      rr in WF. des; clarify; rewrite Any.upcast_downcast in *; clarify.
-      2: { steps. des; clarify. ur in _ASSUME0. des_ifs. }
-      steps. des; clarify. unfold ccallU. steps. force_l. exists (InitX, AppRA.unit, Init).
-      steps. force_l; ss. steps. force_l; ss.
-      { ur; ss. }
-      steps. des; clarify; rewrite Any.upcast_downcast in *; clarify.
-      2: { steps. des; clarify. ur in _ASSUME2. des_ifs. }
-      steps. force_l. exists (RunX, Run, AppRA.unit). steps. force_l; ss. steps. des; clarify.
-      assert(x = AppRA.unit). { ur in _ASSUME2. des_ifs. } subst.
-      force_l; ss.
-      { ur; ss. }
-      steps. rr. esplits; et. rr. right; ss.
+    { init. harg. mDesAll; des; clarify. fold wf. steps. unfold initF, MWApp0.initF, ccallU. steps.
+      mDesOr "INV"; mDesAll; des; clarify; cycle 1.
+      { admit "ez". }
+      rewrite Any.upcast_downcast in *. clarify. steps. force_l; stb_tac; ss; clarify. steps.
+
+      hcall _ _ _ with "INV".
+      { iSplits; ss; et. }
+      { esplits; ss; et. }
+      fold wf. mDesAll; des; clarify.
+      mDesOr "INV1"; mDesAll; des; clarify; cycle 1.
+      { admit "ez". }
+      steps. hret _; ss.
+      { iModIntro. iFrame. iSplits; ss; et. }
     }
     econs; ss.
-    { init. steps. unfold runF, MWApp0.runF, ASSUME, GUARANTEE. steps.
-      rr in WF. des; clarify; rewrite Any.upcast_downcast in *; clarify.
-      1: { steps. des; clarify. ur in _ASSUME0. des_ifs. }
-      steps. des; clarify. unfold ccallU. steps. force_l. exists (RunX, AppRA.unit, Run).
-      steps. force_l; ss. steps. force_l; ss.
-      { ur; ss. }
-      steps. des; clarify; rewrite Any.upcast_downcast in *; clarify.
-      1: { steps. des; clarify. ur in _ASSUME2. des_ifs. }
-      steps. des; clarify. force_l. exists (RunX, Run, AppRA.unit). steps. force_l; ss. steps.
-      assert(x = AppRA.unit). { ur in _ASSUME2. des_ifs. } subst.
-      force_l; ss. steps. rr. esplits; et. rr. right; ss.
+    { init. harg. mDesAll; des; clarify. fold wf. steps. unfold runF, MWApp0.runF, ccallU. steps.
+      mDesOr "INV"; mDesAll; des; clarify.
+      { admit "ez". }
+      rewrite Any.upcast_downcast in *. clarify. steps. force_l; stb_tac; ss; clarify. steps.
+
+      hcall _ _ _ with "INV".
+      { iSplits; ss; et. }
+      { esplits; ss; et. }
+      fold wf. mDesAll; des; clarify.
+      mDesOr "INV1"; mDesAll; des; clarify.
+      { admit "ez". }
+      steps. unfold unint in *. des_ifs. steps.
+      hret _; ss.
+      { iModIntro. iFrame. iSplits; ss; et. }
     }
-    (*   { left. ss. esplits; et. *)
-    (*   des; clarify. *)
-    (*   { rewrite Any.upcast_downcast in *. clarify. steps. *)
-    (*   harg. mDesAll. des; clarify. unfold initF, ccallU. steps. *)
-    (*   mDesOr "INV"; mDesAll; des; clarify. *)
-    (*   2: { mAssertPure False; ss. iCombine "INV A" as "A". iOwnWf "A" as WF0. admit "ez". } *)
-    (*   steps. rewrite Any.upcast_downcast in *. clarify. steps. *)
-    (*   hcall _ _ _ with "INV"; auto. *)
-    (*   { esplits; ss. } *)
-    (*   steps. mDesAll; clarify. mDesOr "INV1"; mDesAll; clarify. *)
-    (*   2: { mAssertPure False; ss. iCombine "INV1 A" as "A". iOwnWf "A" as WF0. admit "ez". } *)
-    (*   rewrite _UNWRAPU. steps. *)
-    (*   mAssert _ with "*". *)
-    (*   { iCombine "A" "INV1" as "A". iApply (OwnM_Upd with "A"). *)
-    (*     instantiate (1:=AppRun ⋅ AppRunX). admit "ez". } *)
-    (*   hret _; ss. *)
-    (*   { iMod "A1". iDestruct "A1" as "[A B]". iFrame. iSplits; ss; et. } *)
-    (* } *)
-    (* econs; ss. *)
-    (* { init. harg. mDesAll. des; clarify. unfold runF, ccallU. steps. *)
-    (*   mDesOr "INV"; mDesAll; des; clarify. *)
-    (*   1: { mAssertPure False; ss. iCombine "INV A" as "A". iOwnWf "A" as WF0. admit "ez". } *)
-    (*   steps. rewrite Any.upcast_downcast in *. clarify. steps. *)
-    (*   hcall _ _ _ with "INV"; auto. *)
-    (*   { esplits; ss. } *)
-    (*   steps. mDesAll; clarify. mDesOr "INV1"; mDesAll; clarify. *)
-    (*   1: { mAssertPure False; ss. iCombine "INV1 A" as "A". iOwnWf "A" as WF0. admit "ez". } *)
-    (*   rewrite _UNWRAPU. steps. *)
-    (*   hret _; ss. *)
-    (*   { iFrame. iSplits; ss; et. } *)
-    (* } *)
   Unshelve. all: ss. all: try exact 0.
   Qed.
 
