examples/mw/MWApp12proof.v
@@ -16,7 +16,7 @@ From ExtLib Require Import
      Structures.Maps
      Data.Map.FMapAList.
 
-Require Import HTactics ProofMode STB.
+Require Import HTactics2 ProofMode STB.
 
 Set Implicit Arguments.
 
@@ -38,7 +38,8 @@ Section SIMMODSEM.
       _
       unit
       (* (fun _ _ mpr_tgt => (∃ (mr_tgt: AppRA), ⌜mpr_tgt = Any.pair tt↑ (GRA.embed mr_tgt)↑⌝ ** OwnM mr_tgt)%I) *)
-      (fun _ _ mpr_tgt => (∃ (rm: AppRA.t), ⌜mpr_tgt = rm↑⌝ ** OwnM rm)%I)
+      (* (fun _ _ mpr_tgt => (∃ (rm: AppRA.t), ⌜mpr_tgt = rm↑⌝ ** OwnM rm)%I) *)
+      (fun _ _ _ => True%I)
   .
 
   Opaque AppRA.t. (****************** todo move to the root ******************)
@@ -51,63 +52,74 @@ Section SIMMODSEM.
   Theorem correct: refines2 [MWApp1.App] [MWApp2.App global_stb].
   Proof.
     eapply adequacy_local2. econs; ss.
-    i. econstructor 1 with (wf:=wf) (le:=top2); et; swap 2 3.
-    { ss. }
-    (* { esplits. econs; ss. eapply to_semantic. iIntros "H". iSplits; ss. } *)
-    { esplits. econs; ss. eapply to_semantic. iIntros "H". iSplits; ss. }
+    i. econstructor 1 with (wf:=wf) (le:=top2); ss.
+    2: { esplits. econs; et. eapply to_semantic. iIntros "A". iFrame. }
 
-    econs; ss.
-    { init. harg. mDesAll. des; clarify. rename x into mwf. rename a into _lower_layer_rm.
-      steps. unfold initF, ASSUME, GUARANTEE. steps.
-      force_r. exists Init. steps. force_r; ss. steps. force_r. eexists. steps. force_r; ss.
-      { esplits; et. admit "ez". }
-      steps. rename c0 into rm. rename c1 into ro. rename c into rf1.
-      rewrite URA.unit_id in _GUARANTEE0.
-      mCombine "A1" "A2". mEval ltac:(erewrite URA.add_comm; erewrite <- _GUARANTEE0) in "A1".
-      unfold ccallU. steps. des. clear_tac. mDesOwn "A1" as "B" "C".
+    econs.
+    {
+      (*** init ***)
+      init.
+      rename mp_tgt into mpr_tgt.
+      assert(exists mp_src mp_tgt (mr_src mr_tgt: Σ),
+                mrp_src = Any.pair mp_src mr_src↑ ∧ mpr_tgt = Any.pair mp_tgt mr_tgt↑).
+      { inv WF. esplits; et. } des; clarify.
+      (*** init ***)
+
+      unfold initF, ccallU.
+      harg. fold wf.
+      mDesAll; des; clarify. steps.
       erewrite STBINCL; cycle 1. { stb_tac; ss. } steps.
-      hcall _ (_, _, _) _ with "A B".
-      { iModIntro. iDestruct "B" as "[B C]". iFrame. iSplits; ss; et. }
+      harg_tgt.
+      { iFrame. iModIntro. iSplits; ss; et. xtra. }
+      steps. stb_tac. clarify.
+      hcall _ _ _.
+      { instantiate (2:=(_,_,_)). cbn. iDes; des; clarify. iDestruct "FR" as "[A B]". iFrame.
+        iModIntro. iSplits; ss; et. instantiate (1:=True%I); ss. }
       { esplits; ss; et. }
-      steps. mDesAll; clarify.
-      rewrite _UNWRAPU. steps. force_r. exists ε. steps. force_r; ss. steps. force_r. rename a into rm0.
-      eexists. steps. force_r; ss.
-      { rewrite URA.unit_id. esplits; et. admit "ez". }
-      steps. des; clarify.
-      mAssert _ with "C A".
-      { iCombine "A" "C" as "A". (* sym in _GUARANTEE. iRewrite _GUARANTEE in "A". *) iExact "A". }
-      mEval ltac:(erewrite <- _GUARANTEE) in "A1".
+      { i. iIntros "H". ss. iDes; des; clarify. }
+      fold wf. mDesAll; des; clarify. steps.
+      hpost_tgt.
+      { iFrame. iModIntro. iSplits; ss; et. xtra. }
+      steps. rewrite _UNWRAPU. steps.
 
       hret _; ss.
-      { iModIntro. iDestruct "A1" as "[[A B] C]". iFrame. iSplitL "A"; et. }
+      { iDestruct "Q" as "[Q %]". subst. iDestruct "FR" as "[A B]". iFrame. iSplits; ss; et. }
+      { iDestruct "Q" as "[Q %]". subst. fold wf in WF0. iPureIntro. r. esplits; et. }
+    }
+
+    econs.
+    {
+      (*** init ***)
+      init.
+      rename mp_tgt into mpr_tgt.
+      assert(exists mp_src mp_tgt (mr_src mr_tgt: Σ),
+                mrp_src = Any.pair mp_src mr_src↑ ∧ mpr_tgt = Any.pair mp_tgt mr_tgt↑).
+      { inv WF. esplits; et. } des; clarify.
+      (*** init ***)
+
+      unfold runF, ccallU.
+      harg. fold wf.
+      mDesAll; des; clarify. steps.
+      erewrite STBINCL; cycle 1. { stb_tac; ss. } steps.
+      harg_tgt.
+      { iFrame. iModIntro. iSplits; ss; et. xtra. }
+      steps. stb_tac. clarify.
+      hcall _ _ _.
+      { instantiate (2:=(_,_,_)). cbn. iDes; des; clarify. iDestruct "FR" as "[A B]". iFrame.
+        iModIntro. iSplits; ss; et. instantiate (1:=True%I); ss. }
+      { esplits; ss; et. }
+      { i. iIntros "H". ss. iDes; des; clarify. }
+      fold wf. mDesAll; des; clarify. steps.
+      hpost_tgt.
+      { iFrame. iModIntro. iSplits; ss; et. xtra. }
+      steps. rewrite _UNWRAPU. steps.
+
+      hret _; ss.
+      { iDestruct "Q" as "[Q %]". subst. iDestruct "FR" as "[A B]". iFrame. iSplits; ss; et. }
+      { iDestruct "Q" as "[Q %]". subst. fold wf in WF0. iPureIntro. r. esplits; et. }
     }
 
     econs; ss.
-    { init. harg. mDesAll. des; clarify. rename x into mwf. rename a into _lower_layer_rm.
-      steps. unfold runF, ASSUME, GUARANTEE. steps.
-      force_r. exists Run. steps. force_r; ss. steps. force_r. eexists. steps. force_r; ss.
-      { esplits; et. admit "ez". }
-      steps. rename c0 into rm. rename c1 into ro. rename c into rf1.
-      rewrite URA.unit_id in _GUARANTEE0.
-      mCombine "A1" "A2". mEval ltac:(erewrite URA.add_comm; erewrite <- _GUARANTEE0) in "A1".
-      unfold ccallU. steps. des. clear_tac. mDesOwn "A1" as "B" "C".
-      erewrite STBINCL; cycle 1. { stb_tac; ss. } steps.
-      hcall _ (_, _, _) _ with "A B".
-      { iModIntro. iDestruct "B" as "[B C]". iFrame. iSplits; ss; et. }
-      { esplits; ss; et. }
-      steps. mDesAll; clarify.
-      rewrite _UNWRAPU. steps. rewrite Any.upcast_downcast in *. clarify. steps.
-      force_r. exists ε. steps. force_r; ss. steps. force_r. rename a into rm0.
-      eexists. steps. force_r; ss.
-      { rewrite URA.unit_id. esplits; et. admit "ez". }
-      steps. des; clarify.
-      mAssert _ with "C A".
-      { iCombine "A" "C" as "A". (* sym in _GUARANTEE. iRewrite _GUARANTEE in "A". *) iExact "A". }
-      mEval ltac:(erewrite <- _GUARANTEE) in "A2".
-
-      hret _; ss.
-      { iModIntro. iDestruct "A2" as "[[A B] C]". iFrame. iSplitL "A"; et. }
-    }
   Unshelve. all: ss. all: try exact 0.
   Qed.
 
